# Pr√°ctica 4 / Ejercicio 2

$\partial_1(10^*1) = \partial_1(1)0^*1 | \epsilon(1)\partial_1(0^*1) = \lambda 0^*1 | \emptyset\partial_1(0^*1) = 0^*1$

$\partial_0(10^*1) = \partial_0(1)0^*1 | \epsilon(1)\partial_0(0^*1) = \emptyset | \emptyset = \emptyset$

$\partial_a(ab^\ast|ac|c^+) = \partial_a(a)b^\ast | \partial_a(ac) | \partial_a(c^+) = \lambda b^\ast | \lambda c | \emptyset = b^\ast | c$

$\partial_a(a^+ba) = \partial_a(a^+) ba | \epsilon(a^+) \partial_a(ba) = \partial_a(aa^\ast) ba | \emptyset \partial_a(ba) = (\partial_a(a) a^\ast | \epsilon(a) \partial_a(a^\ast)) ba = (\lambda a^\ast | \emptyset \partial_a(a^\ast)) ba = a^\ast ba$

$\partial_a(a^\ast ba) = \partial_a(a^\ast) ba | \epsilon(a^\ast) \partial_a(ba) = \partial_a(a) a^\ast ba | \lambda \partial_a(ba) = \lambda a^\ast ba | \lambda \emptyset = a^\ast ba$

$\partial_1(\partial_0(0(1|\lambda)|1^+)) = \partial_1( \partial_0(0) (1|\lambda) | \epsilon(0) \partial_0(1|\lambda) | \partial_0(1^+) ) = \partial_1( \lambda (1|\lambda) | \emptyset \partial_0(1|\lambda) | \emptyset ) = \partial_1(1 | \lambda) = \partial_1(1) \lambda | \epsilon(1) \partial_1(\lambda) = \lambda \lambda | \emptyset \partial_1(\lambda) = \lambda$
