# Práctica 1 / Ejercicio 5

Dado un alfabeto $\Sigma$, sean $x, y \in \Sigma$ y $\alpha, \beta \in \Sigma^*$.

---

**a)** $|x.(y.\alpha)| = 2 + |\alpha|$

$$
\begin{align*}
|x.(y.\alpha)|
&= |x| + |y.\alpha| & \hspace{2em} \text{prop $|\bullet|$} \\
&= |x| + |y| + |\alpha| & \hspace{2em} \text{prop $|\bullet|$} \\
&= 1 + 1 + |\alpha| & \hspace{2em} \text{def $|\bullet|$} \\
&= 2 + |\alpha|
\end{align*}
$$

---

**b)** $|\alpha^r| = |\alpha|$

**Inducción estructural**

Caso base: $\alpha = \lambda$

$$
\begin{align*}
|\alpha^r|
&= |\lambda^r| \\
&= |\lambda| & \hspace{2em} \text{def $\bullet^r$} \\
&= |\alpha|
\end{align*}
$$

Caso inductivo: $\alpha = x\beta$ \
Hipótesis inductiva: $|\beta^r| = |\beta|$

$$
\begin{align*}
|\alpha^r|
&= |(x\beta)^r| \\
&= |\beta^rx| & \hspace{2em} \text{def $\bullet^r$} \\
&= |\beta^r| + 1 & \hspace{2em} \text{def $|\bullet|$} \\
&= |\beta| + 1 & \hspace{2em} \text{HI} \\
&= |x\beta| & \hspace{2em} \text{def $|\bullet|$} \\
&= |\alpha|
\end{align*}
$$

---

**c)** $|\alpha x \beta| = |x \alpha \beta|$

$$
\begin{align*}
|\alpha x\beta|
&= |\alpha| + |x\beta| & \hspace{2em} \text{prop $|\bullet|$} \\
&= |\alpha| + 1 + |\beta| & \hspace{2em} \text{def $|\bullet|$} \\
&= 1 + |\alpha| + |\beta| \\
&= |x\alpha| + |\beta| & \hspace{2em} \text{def $|\bullet|$} \\
&= |x\alpha\beta| & \hspace{2em} \text{prop $|\bullet|$} \\
\end{align*}
$$

---

**d)** $|\alpha.\alpha| = 2|\alpha|$

$$
\begin{align*}
|\alpha.\alpha|
&= |\alpha| + |\alpha| & \hspace{2em} \text{prop $|\bullet|$} \\
&= 2|\alpha|
\end{align*}
$$

---

**e)** $(\alpha.\beta)^r = \beta^r \alpha^r$

**Inducción estructural** (con cualquier $\beta$ fijo)

Caso base: $\alpha = \lambda$

$$
\begin{align*}
(\alpha.\beta)^r
&= (\lambda.\beta)^r \\
&= \beta^r \\
&= \beta^r . \lambda \\
&= \beta^r . \lambda^r & \hspace{2em} \text{def $\bullet^r$} \\
&= \beta^r . \alpha^r
\end{align*}
$$

Caso inductivo: $\alpha = x\gamma$ \
Hipótesis inductiva: $(\gamma.\beta)^r = \beta^r \gamma^r$

$$
\begin{align*}
(\alpha.\beta)^r
&= (x\gamma.\beta)^r \\
&= (\gamma.\beta)^rx & \hspace{2em} \text{def $\bullet^r$} \\
&= \beta^r \gamma^rx & \hspace{2em} \text{HI} \\
&= \beta^r (x\gamma)^r & \hspace{2em} \text{def $\bullet^r$} \\
&= \beta^r \alpha^r
\end{align*}
$$

---

**f)** $(\alpha^r)^r = \alpha$

**Inducción estructural**

Caso base: $\alpha = \lambda$

$$
\begin{align*}
(\alpha^r)^r
&= (\lambda^r)^r \\
&= \lambda^r & \hspace{2em} \text{def $\bullet^r$} \\
&= \lambda & \hspace{2em} \text{def $\bullet^r$} \\
&= \alpha
\end{align*}
$$

Caso inductivo: $\alpha = x\beta$ \
Hipótesis inductiva: $(\beta^r)^r = \beta$

$$
\begin{align*}
(\alpha^r)^r
&= ((x\beta)^r)^r \\
&= (\beta^r x)^r & \hspace{2em} \text{def $\bullet^r$} \\
&= x^r (\beta^r)^r & \hspace{2em} \text{prop $\bullet^r$ (inciso e)} \\
&= x (\beta^r)^r & \hspace{2em} \text{def $\bullet^r$} \\
&= x \beta & \hspace{2em} \text{HI} \\
&= \alpha
\end{align*}
$$

---

**g)** $(\alpha^r)^n = (\alpha^n)^r$

**Inducción en n**

Caso base: $n = 0$

$$
\begin{align*}
(\alpha^r)^n
&= (\alpha^r)^0 \\
&= \lambda & \hspace{2em} \text{def $\bullet^n$} \\
&= \lambda^n \\
&= (\lambda^n)^r \\
&= (\alpha^n)^r
\end{align*}
$$

Caso inductivo: $(\alpha^r)^{n+1}$ \
Hipótesis inductiva: $(\alpha^r)^n = (\alpha^n)^r$

$$
\begin{align*}
(\alpha^r)^{n+1}
&= \alpha^r . (\alpha^r)^n & \hspace{2em} \text{def $\bullet^n$} \\
&= \alpha^r . (\alpha^n)^r & \hspace{2em} \text{HI} \\
&= (\alpha^n . \alpha)^r & \hspace{2em} \text{prop $\bullet^r$} \\
&= (\underbrace{\alpha \dots \alpha \lambda}_{|\bullet|_{\alpha} = n} . \alpha)^r & \hspace{2em} \text{def $\bullet^n$} \\
&= (\underbrace{\alpha \dots \alpha \alpha \lambda}_{|\bullet|_{\alpha} = n+1})^r \\
&= (\alpha^{n+1})^r & \hspace{2em} \text{def $\bullet^n$} \\
\end{align*}
$$
