# Práctica 1 / Ejercicio 10

Sean $\mathcal{L}, \mathcal{L_1}, \mathcal{L_2}$ lenguajes cualesquiera.

---

**a)** $\mathcal{L}^+ \subseteq \mathcal{L}^*$

**Verdadero**

$\mathcal{L}^+ = \bigcup\limits_{i\geq1} \mathcal{L}^i \subseteq \mathcal{L}^* = \bigcup\limits_{i\geq0} \mathcal{L}^i$

---

**b)** $\mathcal{L}^+ \subsetneq \mathcal{L}^*$

**Falso**

$\{ \lambda \}^+ = \{ \lambda \} = \{ \lambda \}^*$

---

**c)** $\mathcal{L}^n \mathcal{L}^m = \mathcal{L}^{n+m}$ para todo $n,m \geq 0$

**Verdadero**

$\mathcal{L}^n \mathcal{L}^m \subseteq \mathcal{L}^{n+m}$

$\alpha \in \mathcal{L}^n \mathcal{L}^m \implies \alpha = \gamma \beta \hspace{1.5em} \gamma \in \mathcal{L}^n \hspace{1.5em} \beta \in \mathcal{L}^m$ \
$\gamma \in \mathcal{L}^n \implies \gamma = \gamma_1 \dots \gamma_n \hspace{1.5em} \gamma_i \in \mathcal{L} \hspace{1.5em} 1 \leq i \leq n$ \
$\beta \in \mathcal{L}^m \implies \beta = \beta_1 \dots \beta_m \hspace{1.5em} \beta_i \in \mathcal{L} \hspace{1.5em} 1 \leq i \leq m$

$\alpha = (\gamma_1 \dots \gamma_n) . (\beta_1 \dots \beta_m) = \alpha_1 \dots \alpha_{n+m} \hspace{1.5em} \alpha_i \in \mathcal{L} \hspace{1.5em} 1 \leq i \leq n+m$ \
$\implies \alpha \in \mathcal{L}^{n+m}$

$\mathcal{L}^n \mathcal{L}^m \supseteq \mathcal{L}^{n+m}$

$\alpha \in \mathcal{L}^{n+m} \implies \alpha = \alpha_1 \dots \alpha_{n+m} \hspace{1.5em} \alpha_i \in \mathcal{L} \hspace{1.5em} 1 \leq i \leq n+m$ \
$\alpha = \underbrace{(\alpha_1 \dots \alpha_n)}_{\gamma} . \underbrace{(\alpha_{n+1} \dots \alpha_{n+m})}_{\beta} = \gamma . \beta$

$\gamma = \alpha_1 \dots \alpha_n = \gamma_1 \dots \gamma_n \hspace{1.5em} \gamma_i = \alpha_i \in \mathcal{L} \hspace{1.5em} 1 \leq i \leq n$ \
$\implies \gamma \in \mathcal{L}^n$

$\beta = \alpha_{n+1} \dots \alpha_{n+m} = \beta_1 \dots \beta_m \hspace{1.5em} \beta_i = \alpha_{n+i} \in \mathcal{L} \hspace{1.5em} 1 \leq i \leq m$ \
$\implies \beta \in \mathcal{L}^m$

$\implies \alpha = \gamma . \beta \in \mathcal{L}^n \mathcal{L}^m$

---

**d)** $\mathcal{L}^n \subseteq \mathcal{L}^{n+1}$ para todo $n \geq 0$

**Falso**: $\{ a \}^n = \{ a^n \} \nsubseteq \{ a^{n+1} \} = \{ a \}^{n+1}$

Solo vale si $\lambda \in \mathcal{L}$.

---

**e)** $\mathcal{L_1} \subseteq \mathcal{L_2}, n \geq 0 \implies (\mathcal{L_1})^n \subseteq (\mathcal{L_2})^n$

**Verdadero**

$\alpha \in (\mathcal{L_1})^n \implies \alpha = \alpha_1 \dots \alpha_n \hspace{1.5em} \alpha_i \in \mathcal{L_1} \hspace{1.5em} 1 \leq i \leq n$ \
$\alpha_i \in \mathcal{L_1} \land \mathcal{L_1} \subseteq \mathcal{L_2} \implies \alpha_i \in \mathcal{L_2} \hspace{1.5em} 1 \leq i \leq n$ \
$\implies \alpha \in (\mathcal{L_2})^n$

---

**f)** $\mathcal{L_1} \subseteq \mathcal{L_2} \implies (\mathcal{L_1})^* \subseteq (\mathcal{L_2})^*$

**Verdadero**

$\alpha \in (\mathcal{L_1})^* = \bigcup\limits_{i \geq 0}^{\infty} (\mathcal{L_1})^i \implies \alpha \in (\mathcal{L_1})^n$ para algún $n \geq 0$

Como $\mathcal{L_1} \subseteq \mathcal{L_2}$, por el inciso d) vale que $\alpha \in (\mathcal{L_2})^n$

$(\mathcal{L_2})^n \subseteq (\mathcal{L_2})^*$ para todo $n \geq 0$ $\implies \alpha \in (\mathcal{L_2})^*$

---

**g)** $(\mathcal{L}^*)^* = \mathcal{L}^*$

**Verdadero**

---

**h)** $(\mathcal{L}^+)^+ = \mathcal{L}^*$

**Falso**

$\mathcal{L} = \{ a \}$ \
$\mathcal{L}^+ = \{ a^n \mid n \geq 1 \}$ \
$(\mathcal{L}^+)^+ = \{ (a^n)^m \mid n,m \geq 1 \} = \{ a^n \mid n \geq 1 \}$ \
$\mathcal{L}^* = \{ a^n \mid n \geq 0 \}$

En particular $\lambda \notin (\mathcal{L}^+)^+$ pero $\lambda \in \mathcal{L}^*$.

---

**i)** $(\mathcal{L}^+)^* = \mathcal{L}^*$

**Verdadero**

---

**j)** $(\mathcal{L_1} \cup \mathcal{L_2})^* = (\mathcal{L_1})^* \cup (\mathcal{L_2})^*$

**Falso**

$\mathcal{L_1} = \{ a \}$ \
$\mathcal{L_2} = \{ b \}$ \
$(\mathcal{L_1})^* = \{ \lambda, a, aa, aaa, \dots \}$ \
$(\mathcal{L_2})^* = \{ \lambda, b, bb, bbb, \dots \}$ \
$(\mathcal{L_1} \cup \mathcal{L_2})^* = \{ a, b \}^* = \{ \lambda, a, b, aa, ab, ba, bb, \dots \}$ \
$ab \in (\mathcal{L_1} \cup \mathcal{L_2})^*$ pero $ab \notin (\mathcal{L_1})^* \cup (\mathcal{L_2})^*$

---

**k)** $(\mathcal{L_1} \cap \mathcal{L_2})^* = (\mathcal{L_1})^* \cap (\mathcal{L_2})^*$

**Falso**

$\mathcal{L_1} = \{ a \}$ \
$\mathcal{L_2} = \{ aa \}$

$(\mathcal{L_1} \cap \mathcal{L_2})^* = \emptyset^* = \Lambda \neq (\mathcal{L_1})^* \cap (\mathcal{L_2})^* = \{ \lambda, a, aa, aaa, aaaa, \dots \} \cap \{ \lambda, aa, aaaa, \dots \} = \{ a^{2n} \mid n \geq 0 \}$

---

**l)** $(\mathcal{L}^2)^* = \mathcal{L}^*$

**Falso**

$\mathcal{L} = \{ a \}$ \
$(\mathcal{L}^2)^* = \{ aa \}^* = \{ \lambda, aa, aaaa, \dots\} = \{ a^{2n} \mid n \geq 0 \} \neq \mathcal{L}^* = \{ a \}^* = \{ \lambda, a, aa, aaa, \dots \} = \{ a^n \mid n \geq 0 \}$

---

**m)** $(\mathcal{L} \cup \mathcal{L}^2)^* = \mathcal{L}^*$

**Verdadero**

---

**n)** $(\mathcal{L}^n)^r = (\mathcal{L}^r)^n$ para todo $n \geq 0$

**Verdadero**

---

**ñ)** $(\mathcal{L}^*)^r = (\mathcal{L}^r)^*$

**Verdadero**
